Weidenbach_Book/IsaSAT/IsaSAT_Show_LLVM.thy
@@ -40,25 +40,20 @@ sepref_def print_char_impl
 
 
 sepref_def isasat_current_information_impl [llvm_code]
-  is \<open>uncurry2 (RETURN ooo isasat_current_information)\<close>
-  :: \<open>word_assn\<^sup>k *\<^sub>a stats_assn\<^sup>k *\<^sub>a lcount_assn\<^sup>k \<rightarrow>\<^sub>a stats_assn\<close>
-  unfolding isasat_current_information_def
+  is \<open>uncurry2 (RETURN ooo isasat_current_information_stats)\<close>
+  :: \<open>word_assn\<^sup>k *\<^sub>a stats_int_assn\<^sup>d *\<^sub>a lcount_assn\<^sup>k \<rightarrow>\<^sub>a stats_int_assn\<close>
+  unfolding isasat_current_information_stats_def
     isasat_current_information_def lcount_assn_def
   by sepref
 
-declare isasat_current_information_impl.refine[sepref_fr_rules]
+lemma isasat_current_information_stats_isasat_current_information:
+  \<open>(isasat_current_information_stats, isasat_current_information) \<in> word_rel \<rightarrow> stats_rel \<rightarrow> Id \<rightarrow> stats_rel\<close>
+  by (auto simp: isasat_current_information_def code_hider_rel_def)
 
-lemma current_restart_phase_alt_def:
-  \<open>current_restart_phase =
-    (\<lambda>(fast_ema, slow_ema, (ccount, ema_lvl, restart_phase, end_of_phase), wasted, \<phi>).
-      restart_phase)\<close>
-  by (auto intro!: ext)
+lemmas [sepref_fr_rules] =
+  isasat_current_information_impl.refine[FCOMP isasat_current_information_stats_isasat_current_information,
+  unfolded stats_assn_alt_def[symmetric]]
 
-sepref_def current_restart_phase_impl
-  is \<open>RETURN o current_restart_phase\<close>
-  :: \<open>heuristic_assn\<^sup>k \<rightarrow>\<^sub>a word_assn\<close>
-  unfolding current_restart_phase_alt_def heuristic_assn_def
-  by sepref
 
 sepref_def isasat_current_status_fast_code
   is \<open>isasat_current_status\<close>
@@ -69,10 +64,19 @@ sepref_def isasat_current_status_fast_code
   by sepref
 
 sepref_def isasat_print_progress_impl
-  is \<open>uncurry3 (RETURN oooo isasat_print_progress)\<close>
-  :: \<open>word_assn\<^sup>k *\<^sub>a word_assn\<^sup>k *\<^sub>a stats_assn\<^sup>k *\<^sub>a lcount_assn\<^sup>k \<rightarrow>\<^sub>a unit_assn\<close>
-  unfolding isasat_print_progress_def lcount_assn_def
+  is \<open>uncurry3 (RETURN oooo isasat_print_progress_stats)\<close>
+  :: \<open>word_assn\<^sup>k *\<^sub>a word_assn\<^sup>k *\<^sub>a stats_int_assn\<^sup>k *\<^sub>a lcount_assn\<^sup>k \<rightarrow>\<^sub>a unit_assn\<close>
+  unfolding isasat_print_progress_stats_def lcount_assn_def
   by sepref
+
+lemma isasat_print_progress_stats_isasat_print_progress:
+  \<open>(uncurry3 (RETURN oooo isasat_print_progress_stats), uncurry3 (RETURN oooo isasat_print_progress))
+  \<in> word_rel \<times>\<^sub>f word_rel \<times>\<^sub>f stats_rel \<times>\<^sub>f Id \<rightarrow> \<langle>unit_rel\<rangle>nres_rel\<close>
+  by (auto simp: isasat_print_progress_def code_hider_rel_def intro!: nres_relI)
+
+lemmas [sepref_fr_rules] =
+  isasat_print_progress_impl.refine[FCOMP isasat_print_progress_stats_isasat_print_progress,
+  unfolded stats_assn_alt_def[symmetric]]
 
 sepref_def isasat_current_progress_impl
   is \<open>uncurry isasat_current_progress\<close>
